add 'global_state' to notion of language

src/program_logic/ectx_language.v
@@ -10,19 +10,19 @@ structure. Use the coercion [LanguageOfEctx] as defined in the bottom of this
 file for doing that. *)
 
 Section ectx_language_mixin.
-  Context {expr val ectx state observation : Type}.
+  Context {expr val ectx state global_state observation : Type}.
   Context (of_val : val → expr).
   Context (to_val : expr → option val).
   Context (empty_ectx : ectx).
   Context (comp_ectx : ectx → ectx → ectx).
   Context (fill : ectx → expr → expr).
-  Context (head_step : expr → state → list observation → expr → state → list expr → Prop).
+  Context (head_step : expr → state → global_state → list observation → expr → state → global_state → list expr → Prop).
 
   Record EctxLanguageMixin := {
     mixin_to_of_val v : to_val (of_val v) = Some v;
     mixin_of_to_val e v : to_val e = Some v → of_val v = e;
-    mixin_val_head_stuck e1 σ1 κ e2 σ2 efs :
-      head_step e1 σ1 κ e2 σ2 efs → to_val e1 = None;
+    mixin_val_head_stuck e1 σ1 g1 κ e2 σ2 g2 efs :
+      head_step e1 σ1 g1 κ e2 σ2 g2 efs → to_val e1 = None;
 
     mixin_fill_empty e : fill empty_ectx e = e;
     mixin_fill_comp K1 K2 e : fill K1 (fill K2 e) = fill (comp_ectx K1 K2) e;
@@ -37,17 +37,17 @@ Section ectx_language_mixin.
 
         This implies there can be only one head redex, see
         [head_redex_unique]. *)
-    mixin_step_by_val K' K_redex e1' e1_redex σ1 κ e2 σ2 efs :
+    mixin_step_by_val K' K_redex e1' e1_redex σ1 g1 κ e2 σ2 g2 efs :
       fill K' e1' = fill K_redex e1_redex →
       to_val e1' = None →
-      head_step e1_redex σ1 κ e2 σ2 efs →
+      head_step e1_redex σ1 g1 κ e2 σ2 g2 efs →
       ∃ K'', K_redex = comp_ectx K' K'';
 
     (** If [fill K e] takes a head step, then either [e] is a value or [K] is
         the empty evaluation context. In other words, if [e] is not a value
         wrapping it in a context does not add new head redex positions. *)
-    mixin_head_ctx_step_val K e σ1 κ e2 σ2 efs :
-      head_step (fill K e) σ1 κ e2 σ2 efs → is_Some (to_val e) ∨ K = empty_ectx;
+    mixin_head_ctx_step_val K e σ1 g1 κ e2 σ2 g2 efs :
+      head_step (fill K e) σ1 g1 κ e2 σ2 g2 efs → is_Some (to_val e) ∨ K = empty_ectx;
   }.
 End ectx_language_mixin.
 
@@ -56,6 +56,7 @@ Structure ectxLanguage := EctxLanguage {
   val : Type;
   ectx : Type;
   state : Type;
+  global_state : Type;
   observation : Type;
 
   of_val : val → expr;
@@ -63,7 +64,7 @@ Structure ectxLanguage := EctxLanguage {
   empty_ectx : ectx;
   comp_ectx : ectx → ectx → ectx;
   fill : ectx → expr → expr;
-  head_step : expr → state → list observation → expr → state → list expr → Prop;
+  head_step : expr → state → global_state → list observation → expr → state → global_state → list expr → Prop;
 
   ectx_language_mixin :
     EctxLanguageMixin of_val to_val empty_ectx comp_ectx fill head_step
@@ -72,7 +73,7 @@ Structure ectxLanguage := EctxLanguage {
 Bind Scope expr_scope with expr.
 Bind Scope val_scope with val.
 
-Global Arguments EctxLanguage {_ _ _ _ _ _ _ _ _ _ _} _.
+Global Arguments EctxLanguage {_ _ _ _ _ _ _ _ _ _ _ _} _.
 Global Arguments of_val {_} _.
 Global Arguments to_val {_} _.
 Global Arguments empty_ectx {_}.
@@ -88,7 +89,8 @@ Section ectx_language.
   Implicit Types K : ectx Λ.
 
   (* Only project stuff out of the mixin that is not also in language *)
-  Lemma val_head_stuck e1 σ1 κ e2 σ2 efs : head_step e1 σ1 κ e2 σ2 efs → to_val e1 = None.
+  Lemma val_head_stuck e1 σ1 g1 κ e2 σ2 g2 efs :
+    head_step e1 σ1 g1 κ e2 σ2 g2 efs → to_val e1 = None.
   Proof. apply ectx_language_mixin. Qed.
   Lemma fill_empty e : fill empty_ectx e = e.
   Proof. apply ectx_language_mixin. Qed.
@@ -98,38 +100,38 @@ Section ectx_language.
   Proof. apply ectx_language_mixin. Qed.
   Lemma fill_val K e : is_Some (to_val (fill K e)) → is_Some (to_val e).
   Proof. apply ectx_language_mixin. Qed.
-  Lemma step_by_val K' K_redex e1' e1_redex σ1 κ e2 σ2 efs :
+  Lemma step_by_val K' K_redex e1' e1_redex σ1 g1 κ e2 σ2 g2 efs :
       fill K' e1' = fill K_redex e1_redex →
       to_val e1' = None →
-      head_step e1_redex σ1 κ e2 σ2 efs →
+      head_step e1_redex σ1 g1 κ e2 σ2 g2 efs →
       ∃ K'', K_redex = comp_ectx K' K''.
   Proof. apply ectx_language_mixin. Qed.
-  Lemma head_ctx_step_val K e σ1 κ e2 σ2 efs :
-    head_step (fill K e) σ1 κ e2 σ2 efs → is_Some (to_val e) ∨ K = empty_ectx.
+  Lemma head_ctx_step_val K e σ1 g1 κ e2 σ2 g2 efs :
+    head_step (fill K e) σ1 g1 κ e2 σ2 g2 efs → is_Some (to_val e) ∨ K = empty_ectx.
   Proof. apply ectx_language_mixin. Qed.
 
-  Definition head_reducible (e : expr Λ) (σ : state Λ) :=
-    ∃ κ e' σ' efs, head_step e σ κ e' σ' efs.
-  Definition head_reducible_no_obs (e : expr Λ) (σ : state Λ) :=
-    ∃ e' σ' efs, head_step e σ [] e' σ' efs.
-  Definition head_irreducible (e : expr Λ) (σ : state Λ) :=
-    ∀ κ e' σ' efs, ¬head_step e σ κ e' σ' efs.
-  Definition head_stuck (e : expr Λ) (σ : state Λ) :=
-    to_val e = None ∧ head_irreducible e σ.
+  Definition head_reducible (e : expr Λ) (σ : state Λ) (g : global_state Λ) :=
+    ∃ κ e' σ' g' efs, head_step e σ g κ e' σ' g' efs.
+  Definition head_reducible_no_obs (e : expr Λ) (σ : state Λ) (g : global_state Λ) :=
+    ∃ e' σ' g' efs, head_step e σ g [] e' σ' g' efs.
+  Definition head_irreducible (e : expr Λ) (σ : state Λ) (g : global_state Λ) :=
+    ∀ κ e' σ' g' efs, ¬head_step e σ g κ e' σ' g' efs.
+  Definition head_stuck (e : expr Λ) (σ : state Λ) (g : global_state Λ) :=
+    to_val e = None ∧ head_irreducible e σ g.
 
   (* All non-value redexes are at the root.  In other words, all sub-redexes are
      values. *)
   Definition sub_redexes_are_values (e : expr Λ) :=
     ∀ K e', e = fill K e' → to_val e' = None → K = empty_ectx.
 
-  Inductive prim_step (e1 : expr Λ) (σ1 : state Λ) (κ : list (observation Λ))
-      (e2 : expr Λ) (σ2 : state Λ) (efs : list (expr Λ)) : Prop :=
+  Inductive prim_step (e1 : expr Λ) (σ1 : state Λ) (g1 : global_state Λ) (κ : list (observation Λ))
+      (e2 : expr Λ) (σ2 : state Λ) (g2 : global_state Λ) (efs : list (expr Λ)) : Prop :=
     Ectx_step K e1' e2' :
       e1 = fill K e1' → e2 = fill K e2' →
-      head_step e1' σ1 κ e2' σ2 efs → prim_step e1 σ1 κ e2 σ2 efs.
+      head_step e1' σ1 g1 κ e2' σ2 g2 efs → prim_step e1 σ1 g1 κ e2 σ2 g2 efs.
 
-  Lemma Ectx_step' K e1 σ1 κ e2 σ2 efs :
-    head_step e1 σ1 κ e2 σ2 efs → prim_step (fill K e1) σ1 κ (fill K e2) σ2 efs.
+  Lemma Ectx_step' K e1 σ1 g1 κ e2 σ2 g2 efs :
+    head_step e1 σ1 g1 κ e2 σ2 g2 efs → prim_step (fill K e1) σ1 g1 κ (fill K e2) σ2 g2 efs.
   Proof. econstructor; eauto. Qed.
 
   Definition ectx_lang_mixin : LanguageMixin of_val to_val prim_step.
@@ -137,25 +139,25 @@ Section ectx_language.
     split.
     - apply ectx_language_mixin.
     - apply ectx_language_mixin.
-    - intros ?????? [??? -> -> ?%val_head_stuck].
+    - intros ???????? [??? -> -> ?%val_head_stuck].
       apply eq_None_not_Some. by intros ?%fill_val%eq_None_not_Some.
   Qed.
 
   Canonical Structure ectx_lang : language := Language ectx_lang_mixin.
 
   Definition head_atomic (a : atomicity) (e : expr Λ) : Prop :=
-    ∀ σ κ e' σ' efs,
-      head_step e σ κ e' σ' efs →
-      if a is WeaklyAtomic then irreducible e' σ' else is_Some (to_val e').
+    ∀ σ g κ e' σ' g' efs,
+      head_step e σ g κ e' σ' g' efs →
+      if a is WeaklyAtomic then irreducible e' σ' g' else is_Some (to_val e').
 
   (** * Some lemmas about this language *)
   Lemma fill_not_val K e : to_val e = None → to_val (fill K e) = None.
   Proof. rewrite !eq_None_not_Some. eauto using fill_val. Qed.
 
-  Lemma head_reducible_no_obs_reducible e σ :
-    head_reducible_no_obs e σ → head_reducible e σ.
-  Proof. intros (?&?&?&?). eexists. eauto. Qed.
-  Lemma not_head_reducible e σ : ¬head_reducible e σ ↔ head_irreducible e σ.
+  Lemma head_reducible_no_obs_reducible e σ g :
+    head_reducible_no_obs e σ g → head_reducible e σ g.
+  Proof. intros (?&?&?&?&?). eexists. eauto. Qed.
+  Lemma not_head_reducible e σ g : ¬head_reducible e σ g ↔ head_irreducible e σ g.
   Proof. unfold head_reducible, head_irreducible. naive_solver. Qed.
 
   (** The decomposition into head redex and context is unique.
@@ -163,74 +165,75 @@ Section ectx_language.
       In all sensible instances, [comp_ectx K' empty_ectx] will be the same as
       [K'], so the conclusion is [K = K' ∧ e = e'], but we do not require a law
       to actually prove that so we cannot use that fact here. *)
-  Lemma head_redex_unique K K' e e' σ :
+  Lemma head_redex_unique K K' e e' σ g :
     fill K e = fill K' e' →
-    head_reducible e σ →
-    head_reducible e' σ →
+    head_reducible e σ g →
+    head_reducible e' σ g →
     K = comp_ectx K' empty_ectx ∧ e = e'.
   Proof.
-    intros Heq (κ & e2 & σ2 & efs & Hred) (κ' & e2' & σ2' & efs' & Hred').
+    intros Heq (κ & e2 & σ2 & g2 & efs & Hred) (κ' & e2' & σ2' & g2' & efs' & Hred').
     edestruct (step_by_val K' K e' e) as [K'' HK];
       [by eauto using val_head_stuck..|].
     subst K. move: Heq. rewrite -fill_comp. intros <-%(inj (fill _)).
-    destruct (head_ctx_step_val _ _ _ _ _ _ _ Hred') as [[]%not_eq_None_Some|HK''].
+    destruct (head_ctx_step_val _ _ _ _ _ _ _ _ _ Hred') as [[]%not_eq_None_Some|HK''].
     { by eapply val_head_stuck. }
     subst K''. rewrite fill_empty. done.
   Qed.
 
-  Lemma head_prim_step e1 σ1 κ e2 σ2 efs :
-    head_step e1 σ1 κ e2 σ2 efs → prim_step e1 σ1 κ e2 σ2 efs.
+  Lemma head_prim_step e1 σ1 g1 κ e2 σ2 g2 efs :
+    head_step e1 σ1 g1 κ e2 σ2 g2 efs → prim_step e1 σ1 g1 κ e2 σ2 g2 efs.
   Proof. apply Ectx_step with empty_ectx; by rewrite ?fill_empty. Qed.
 
-  Lemma head_step_not_stuck e σ κ e' σ' efs : head_step e σ κ e' σ' efs → not_stuck e σ.
+  Lemma head_step_not_stuck e σ g κ e' σ' g' efs :
+    head_step e σ g κ e' σ' g' efs → not_stuck e σ g.
   Proof. rewrite /not_stuck /reducible /=. eauto 10 using head_prim_step. Qed.
 
-  Lemma fill_prim_step K e1 σ1 κ e2 σ2 efs :
-    prim_step e1 σ1 κ e2 σ2 efs → prim_step (fill K e1) σ1 κ (fill K e2) σ2 efs.
+  Lemma fill_prim_step K e1 σ1 g1 κ e2 σ2 g2 efs :
+    prim_step e1 σ1 g1 κ e2 σ2 g2 efs → prim_step (fill K e1) σ1 g1 κ (fill K e2) σ2 g2 efs.
   Proof.
     destruct 1 as [K' e1' e2' -> ->].
     rewrite !fill_comp. by econstructor.
   Qed.
-  Lemma fill_reducible K e σ : reducible e σ → reducible (fill K e) σ.
+  Lemma fill_reducible K e σ g : reducible e σ g → reducible (fill K e) σ g.
   Proof.
-    intros (κ&e'&σ'&efs&?). exists κ, (fill K e'), σ', efs.
+    intros (κ&e'&σ'&g'&efs&?). exists κ, (fill K e'), σ', g', efs.
     by apply fill_prim_step.
   Qed.
-  Lemma fill_reducible_no_obs K e σ : reducible_no_obs e σ → reducible_no_obs (fill K e) σ.
+  Lemma fill_reducible_no_obs K e σ g : reducible_no_obs e σ g → reducible_no_obs (fill K e) σ g.
   Proof.
-    intros (e'&σ'&efs&?). exists (fill K e'), σ', efs.
+    intros (e'&σ'&g'&efs&?). exists (fill K e'), σ', g', efs.
     by apply fill_prim_step.
   Qed.
-  Lemma head_prim_reducible e σ : head_reducible e σ → reducible e σ.
-  Proof. intros (κ&e'&σ'&efs&?). eexists κ, e', σ', efs. by apply head_prim_step. Qed.
-  Lemma head_prim_fill_reducible e K σ :
-    head_reducible e σ → reducible (fill K e) σ.
+  Lemma head_prim_reducible e σ g : head_reducible e σ g → reducible e σ g.
+  Proof. intros (κ&e'&σ'&g'&efs&?). eexists κ, e', σ', g', efs. by apply head_prim_step. Qed.
+  Lemma head_prim_fill_reducible e K σ g :
+    head_reducible e σ g → reducible (fill K e) σ g.
   Proof. intro. by apply fill_reducible, head_prim_reducible. Qed.
-  Lemma head_prim_reducible_no_obs e σ : head_reducible_no_obs e σ → reducible_no_obs e σ.
-  Proof. intros (e'&σ'&efs&?). eexists e', σ', efs. by apply head_prim_step. Qed.
-  Lemma head_prim_irreducible e σ : irreducible e σ → head_irreducible e σ.
+  Lemma head_prim_reducible_no_obs e σ g : head_reducible_no_obs e σ g → reducible_no_obs e σ g.
+  Proof. intros (e'&σ'&g'&efs&?). eexists e', σ', g', efs. by apply head_prim_step. Qed.
+  Lemma head_prim_irreducible e σ g : irreducible e σ g → head_irreducible e σ g.
   Proof.
     rewrite -not_reducible -not_head_reducible. eauto using head_prim_reducible.
   Qed.
-  Lemma head_prim_fill_reducible_no_obs e K σ :
-    head_reducible_no_obs e σ → reducible_no_obs (fill K e) σ.
+  Lemma head_prim_fill_reducible_no_obs e K σ g :
+    head_reducible_no_obs e σ g → reducible_no_obs (fill K e) σ g.
   Proof. intro. by apply fill_reducible_no_obs, head_prim_reducible_no_obs. Qed.
 
-  Lemma prim_head_reducible e σ :
-    reducible e σ → sub_redexes_are_values e → head_reducible e σ.
+  Lemma prim_head_reducible e σ g :
+    reducible e σ g → sub_redexes_are_values e → head_reducible e σ g.
   Proof.
-    intros (κ&e'&σ'&efs&[K e1' e2' -> -> Hstep]) ?.
+    intros (κ&e'&σ'&g'&efs&[K e1' e2' -> -> Hstep]) ?.
     assert (K = empty_ectx) as -> by eauto 10 using val_head_stuck.
-    rewrite fill_empty /head_reducible; eauto.
+    rewrite fill_empty /head_reducible; eauto 10.
   Qed.
-  Lemma prim_head_irreducible e σ :
-    head_irreducible e σ → sub_redexes_are_values e → irreducible e σ.
+  Lemma prim_head_irreducible e σ g :
+    head_irreducible e σ g → sub_redexes_are_values e → irreducible e σ g.
   Proof.
     rewrite -not_reducible -not_head_reducible. eauto using prim_head_reducible.
   Qed.
 
-  Lemma head_stuck_stuck e σ :
-    head_stuck e σ → sub_redexes_are_values e → stuck e σ.
+  Lemma head_stuck_stuck e σ g :
+    head_stuck e σ g → sub_redexes_are_values e → stuck e σ g.
   Proof.
     intros [] ?. split; first done.
     by apply prim_head_irreducible.
@@ -239,17 +242,17 @@ Section ectx_language.
   Lemma ectx_language_atomic a e :
     head_atomic a e → sub_redexes_are_values e → Atomic a e.
   Proof.
-    intros Hatomic_step Hatomic_fill σ κ e' σ' efs [K e1' e2' -> -> Hstep].
+    intros Hatomic_step Hatomic_fill σ g κ e' σ' g' efs [K e1' e2' -> -> Hstep].
     assert (K = empty_ectx) as -> by eauto 10 using val_head_stuck.
     rewrite fill_empty. eapply Hatomic_step. by rewrite fill_empty.
   Qed.
 
-  Lemma head_reducible_prim_step_ctx K e1 σ1 κ e2 σ2 efs :
-    head_reducible e1 σ1 →
-    prim_step (fill K e1) σ1 κ e2 σ2 efs →
-    ∃ e2', e2 = fill K e2' ∧ head_step e1 σ1 κ e2' σ2 efs.
+  Lemma head_reducible_prim_step_ctx K e1 σ1 g1 κ e2 σ2 g2 efs :
+    head_reducible e1 σ1 g1 →
+    prim_step (fill K e1) σ1 g1 κ e2 σ2 g2 efs →
+    ∃ e2', e2 = fill K e2' ∧ head_step e1 σ1 g1 κ e2' σ2 g2 efs.
   Proof.
-    intros (κ'&e2''&σ2''&efs''&HhstepK) [K' e1' e2' HKe1 -> Hstep].
+    intros (κ'&e2''&σ2''&g2''&efs''&HhstepK) [K' e1' e2' HKe1 -> Hstep].
     edestruct (step_by_val K) as [K'' ?];
       eauto using val_head_stuck; simplify_eq/=.
     rewrite -fill_comp in HKe1; simplify_eq.
@@ -259,10 +262,10 @@ Section ectx_language.
     by rewrite !fill_empty.
   Qed.
 
-  Lemma head_reducible_prim_step e1 σ1 κ e2 σ2 efs :
-    head_reducible e1 σ1 →
-    prim_step e1 σ1 κ e2 σ2 efs →
-    head_step e1 σ1 κ e2 σ2 efs.
+  Lemma head_reducible_prim_step e1 σ1 g1 κ e2 σ2 g2 efs :
+    head_reducible e1 σ1 g1 →
+    prim_step e1 σ1 g1 κ e2 σ2 g2 efs →
+    head_step e1 σ1 g1 κ e2 σ2 g2 efs.
   Proof.
     intros.
     edestruct (head_reducible_prim_step_ctx empty_ectx) as (?&?&?);
@@ -275,27 +278,27 @@ Section ectx_language.
   Proof.
     split; simpl.
     - eauto using fill_not_val.
-    - intros ?????? [K' e1' e2' Heq1 Heq2 Hstep].
+    - intros ???????? [K' e1' e2' Heq1 Heq2 Hstep].
       by exists (comp_ectx K K') e1' e2'; rewrite ?Heq1 ?Heq2 ?fill_comp.
-    - intros e1 σ1 κ e2 σ2 efs Hnval [K'' e1'' e2'' Heq1 -> Hstep].
-      destruct (step_by_val K K'' e1 e1'' σ1 κ e2'' σ2 efs) as [K' ->]; eauto.
+    - intros e1 σ1 g1 κ e2 σ2 g2 efs Hnval [K'' e1'' e2'' Heq1 -> Hstep].
+      destruct (step_by_val K K'' e1 e1'' σ1 g1 κ e2'' σ2 g2 efs) as [K' ->]; eauto.
       rewrite -fill_comp in Heq1; apply (inj (fill _)) in Heq1.
       exists (fill K' e2''); rewrite -fill_comp; split; auto.
       econstructor; eauto.
   Qed.
 
   Record pure_head_step (e1 e2 : expr Λ) := {
-    pure_head_step_safe σ1 : head_reducible_no_obs e1 σ1;
-    pure_head_step_det σ1 κ e2' σ2 efs :
-      head_step e1 σ1 κ e2' σ2 efs → κ = [] ∧ σ2 = σ1 ∧ e2' = e2 ∧ efs = []
+    pure_head_step_safe σ1 g1 : head_reducible_no_obs e1 σ1 g1;
+    pure_head_step_det σ1 g1 κ e2' σ2 g2 efs :
+      head_step e1 σ1 g1 κ e2' σ2 g2 efs → κ = [] ∧ σ2 = σ1 ∧ g2 = g1 ∧ e2' = e2 ∧ efs = []
   }.
 
   Lemma pure_head_step_pure_step e1 e2 : pure_head_step e1 e2 → pure_step e1 e2.
   Proof.
     intros [Hp1 Hp2]. split.
-    - intros σ. destruct (Hp1 σ) as (e2' & σ2 & efs & ?).
-      eexists e2', σ2, efs. by apply head_prim_step.
-    - intros σ1 κ e2' σ2 efs ?%head_reducible_prim_step; eauto using head_reducible_no_obs_reducible.
+    - intros σ g. destruct (Hp1 σ g) as (e2' & σ2 & g2 & efs & ?).
+      eexists e2', σ2, g2, efs. by apply head_prim_step.
+    - intros σ1 g1 κ e2' σ2 g2 efs ?%head_reducible_prim_step; eauto using head_reducible_no_obs_reducible.
   Qed.
 
   (** This is not an instance because HeapLang's [wp_pure] tactic already takes
@@ -310,7 +313,7 @@ Section ectx_language.
 End ectx_language.
 
 Global Arguments ectx_lang : clear implicits.
-Global Arguments Ectx_step {Λ e1 σ1 κ e2 σ2 efs}.
+Global Arguments Ectx_step {Λ e1 σ1 g1 κ e2 σ2 g2 efs}.
 Coercion ectx_lang : ectxLanguage >-> language.
 
 (* This definition makes sure that the fields of the [language] record do not
@@ -321,6 +324,6 @@ work.
 Note that this trick no longer works when we switch to canonical projections
 because then the pattern match [let '...] will be desugared into projections. *)
 Definition LanguageOfEctx (Λ : ectxLanguage) : language :=
-  let '@EctxLanguage E V C St K of_val to_val empty comp fill head mix := Λ in
-  @Language E V St K of_val to_val _
-    (@ectx_lang_mixin (@EctxLanguage E V C St K of_val to_val empty comp fill head mix)).
+  let '@EctxLanguage E V C St GSt K of_val to_val empty comp fill head mix := Λ in
+  @Language E V St GSt K of_val to_val _
+    (@ectx_lang_mixin (@EctxLanguage E V C St GSt K of_val to_val empty comp fill head mix)).
